### 7.3.4 Analytical Expression of Dot Product $\underline{u}, \underline{v}$ (Dot product of vectors in their components form)

Let $\underline{u}=a_{1} \underline{i}+b_{1} \underline{j}+c_{1} \underline{k}$ and $\underline{v}=a_{2} \underline{i}+b_{2} \underline{j}+c_{2} \underline{k}$
be two non-zero vectors.
From distributive Law we can write:

$$
\begin{aligned}
\therefore \quad \underline{u}, \underline{v}= & \left(a_{1} \underline{i}+b_{1} \underline{j}+c_{1} \underline{k}\right)\left(a_{2} \underline{i}+b_{2} \underline{j}+c_{2} \underline{k}\right) \\
= & a_{1} a_{2}(\underline{i}, \underline{i})+a_{2} b_{1}(\underline{i}, \underline{j})+a_{1} c_{1}(\underline{i}, \underline{k}) \\
& +b_{1} a_{2}(\underline{j}, \underline{i})+b_{1} b_{2}(\underline{j}, \underline{j})+b_{1} c_{2}(\underline{j}, \underline{k}) \\
& +c_{1} a_{2}(\underline{k}, \underline{i})+c_{2} b_{2}(\underline{k}, \underline{j})+c_{1} c_{2}(\underline{k}, \underline{k})
\end{aligned}
$$

$$
\Rightarrow \underline{u}, \underline{v}=a_{1} a_{2}+b_{1} b_{2}+c_{1} c_{2}
$$

Hence the dot product of two vectors is the sum of the product of their corresponding components.
Equivalence of two definitions of dot product of two vectors has been proved in the following example.

Example 1: (i) If $\underline{v}=\left[\underline{x}_{1}, \underline{y}_{1}\right]$ and $\underline{w}=\left[\underline{x}_{2}, \underline{y}_{2}\right]$ are two vectors in the plane, then
$\underline{v}, \underline{w}=\underline{x}_{1} \underline{x}_{2}+\underline{y}_{1} \underline{y}_{2}$
(ii) If $\underline{v}$ and $\underline{w}$ are two non-zero vectors in the plane, then
$\underline{v}, \underline{w}=\underline{\underline{x}} \underline{\underline{x}} \underline{\underline{x}} \cos \theta$
where $\theta$ is the angle between $\underline{v}$ and $\underline{w}$ and $0 \leq \theta \leq \pi$.
Proof: Let $\underline{v}$ and $\underline{w}$ determine the sides of a triangle then the third side, opposite to the angle $\theta$, has length $\mid \underline{v}-\underline{w} \mid$ (by triangle law of addition of vectors)

By law of cosines,

$$
\begin{aligned}
& \mid \underline{v}-\underline{w} \mid^{2}=\left|\underline{v}\right|^{2}+\left|\underline{w}\right|^{2}-2\left|\underline{v}\right| \mid \underline{w} \cos \theta \\
& \text { if } \quad \underline{v}=\left[\underline{x}_{1}, \underline{y}_{1}\right] \text { and } \underline{w}\left[\underline{x}_{2}, \underline{y}_{2}\right], \text { then } \\
& \underline{v}-\underline{w}=\left[\underline{x}_{1}-\underline{x}_{2}, \underline{y}_{1}-\underline{y}_{2}\right]
\end{aligned}
$$

So equation (1) becomes:

$$
\begin{aligned}
& \left|\underline{x}_{1}-\underline{x}_{2}\right|^{2}+\left|\underline{y}_{1}-\underline{y}_{2}\right|^{2}=\left|\underline{x}_{1}^{2}+\underline{y}_{1}^{2}\right|+\left|\underline{x}_{2}^{2}+\underline{y}_{2}^{2}\right|-2\left|\underline{v}\right| \mid \underline{w} \cos \theta \\
& -2 \underline{x}_{1} \underline{x}_{2}-2 \underline{y}_{1} \underline{y}_{2}=2\left|\underline{v}\right| \mid \underline{w} \cos \theta \\
& \Rightarrow \quad \underline{x}_{1} \underline{x}_{2}+\underline{y}_{1} \underline{y}_{2}=\left|\underline{v}\right| \mid \underline{w} \cos \theta=\underline{v}, \underline{w}
\end{aligned}
$$

Example 2: If $\underline{u}=3 \underline{i}-\underline{j}-2 \underline{k}$ and $\underline{v}=\underline{i}+2 \underline{j}-\underline{k}$, then
$\underline{u}, \underline{v}=(-3)(1)+(-1)(2)+(-2)(-1)=3$
Example 3: If $\underline{u}=2 \underline{i}-4 \underline{j}+5 \underline{k}$ and $\underline{v}=-4 \underline{i}-3 \underline{j}-4 \underline{k}$, then
$\underline{u}, \underline{v}=(2)(4)+(-4)(-3)+(5)(-4)=0$
$\Rightarrow \underline{u}$ and $\underline{v}$ are perpendicular