### 7.3.6 Projection of one Vector upon another Vector:

In many physical applications, it is required to know "how much" of a vector is applied along a given direction. For this purpose we find the projection of one vector along the other vector.

Let $\overline{O A}=\underline{u}$ and $\overline{O B}=\gamma$
Let $\theta$ be the angle between them, such that $0 \leq \theta \leq \pi$.
Draw $\overline{B M} \perp O A$. Then $\overline{O M}$ is called the projection of $\chi$ along $\mu$.

$$
\begin{aligned}
& \text { Now } \quad \frac{\overline{O M}}{\overline{O B}}=\cos \theta \text {, that is, } \\
& \overline{O M}=\|\overline{O B}\| \cos \theta=\|\underline{\underline{x}}\| \cos \theta
\end{aligned}
$$

By definition, $\cos \theta=\frac{\underline{\underline{u}} \cdot \underline{\underline{v}}}{\|\underline{\underline{u}}\| \underline{\underline{v}}}$
From (1) and (2), $\overline{O M}=\|\underline{\underline{x}}\| \frac{\underline{\underline{u}} \cdot \underline{\underline{v}}}{\|\underline{\underline{u}}\| \underline{\underline{v}}}\|}$

Projection of $\underline{\underline{v}}$ along $\underline{\underline{u}}=\frac{\underline{\underline{u}} \cdot \underline{\underline{v}}}{\|\underline{\underline{u}}\|}$
Similarly, projection of $\underline{\underline{u}}$ along $\underline{\underline{v}}=\frac{\underline{\underline{u}} \cdot \underline{\underline{v}}}{\|\underline{\underline{v}}\|}$

Example 7: Show that the components of a vector are the projections of that vector along $\underline{i}, \underline{j}$ and $\underline{k}$ respectively.

Solution: Let $\underline{\underline{v}}=a \underline{i}+b \underline{j}+c \underline{k}$, then
Projection of $\underline{\underline{v}}$ along $\underline{i}=\frac{\underline{v} \cdot \underline{j}}{\|\underline{\underline{i}}\|}=\left(a \underline{i}+b \underline{j}+c \underline{k}\right) \cdot \underline{i}=a$
Projection of $\underline{\underline{v}}$ along $\underline{j}=\frac{\underline{v} \cdot \underline{j}}{\|\underline{\underline{j}}\|}=\left(a \underline{i}+b \underline{j}+c \underline{k}\right) \cdot \underline{j}=b$
Projection of $\underline{\underline{v}}$ along $\underline{k}=\frac{\underline{v} \cdot \underline{k}}{\|\underline{\underline{k}}\|}=\left(a \underline{i}+b \underline{j}+c \underline{k}\right) \cdot \underline{k}=c$
Hence components $a, b$ and $c$ of vector $\underline{\underline{v}}=a \underline{i}+b \underline{j}+c \underline{k}$ are projections of vector $\underline{\underline{v}}$ along $\underline{i}, \underline{j}$ and $\underline{k}$ respectively.

Example 8: Prove that in any triangle $A B C$
(i) $a^{2}=b^{2}+c^{2}-2 b c \cos A$
(ii) $a=b \cos C+c \cos B$

## (Cosine Law)

(Projection Law)

Solution: Let the vectors $\underline{a}, \underline{b}$ and $\underline{c}$ be along the sides $B C, C A$ and $A B$ of the triangle $A B C$ as shown in the figure.
$\therefore \quad \underline{a}+\underline{b}+\underline{c}=\underline{0}$
$\Rightarrow \quad \underline{a}=-(\underline{b}+\underline{c})$
Now $\underline{a} \cdot \underline{a}=(\underline{b}+\underline{c}) \cdot(\underline{b}+\underline{c})$
$\Rightarrow \quad=b \cdot b+b \cdot c+c \cdot b+c \cdot c$
$\Rightarrow \quad a^{2}=b^{2}+2 \underline{b} \cdot \underline{c}+c^{2}$
$\Rightarrow \quad a^{2}=b^{2}+c^{2}+2 b c \cdot \cos (\pi-A)$
$\therefore \quad a^{2}=b^{2}+c^{2}-2 b c \cos A$
(ii) $\quad \underline{a}+\underline{b}+\underline{c}=\underline{0}$
$\Rightarrow \quad \underline{a}=-\underline{b}-\underline{c}$
Take dot product with $\underline{a}$
$\underline{a} \cdot \underline{a}=-\underline{a} \cdot \underline{b}-\underline{a} \cdot \underline{c}$
$=-a b \cos (\pi-C)-a c \cos (\pi-B)$
$a^{2}=a b \cos C+a c \cos B$
$\Rightarrow a=b \cos C+c \cos B$
Example 9: Prove that: $\cos (\alpha-\beta)=\cos \alpha \cos \beta+\sin \alpha \sin \beta$
Solution: Let $\overline{O A}$ and $\overline{O B}$ be the unit vectors in the $x y$-plane making angles $\alpha$ and $\beta$ with the positive $x$-axis.

$$
\begin{aligned}
& \text { So that } \angle A O B=\alpha-\beta \\
& \text { Now } \overline{O A}=\cos \alpha \underline{i}+\sin \alpha \underline{j} \\
& \text { and } \overline{O B}=\cos \beta \underline{i}+\sin \beta \underline{j} \\
& \therefore \overline{O A} \cdot \overline{O B}=(\cos \alpha \underline{i}+\sin \alpha \underline{j}) \cdot(\cos \beta \underline{i}+\sin \beta \underline{j}) \\
& \Rightarrow \quad\|\overline{O A}\| \overline{O B} \cdot \cos (\alpha-\beta)=\cos \alpha \cos \beta+\sin \alpha \sin \beta \\
& \therefore \cos (\alpha-\beta)=\cos \alpha \cos \beta+\sin \alpha \sin \beta
\end{aligned}
$$

$(\because \mid \overline{O A} \mid=\mid \overline{O B} \mid=1)$

## EXERCISE 7.3

1. Find the cosine of the angle $\theta$ between $\mu$ and $\gamma$ :
(i) $\mu=3 i+j-k, \gamma=2 i-j+k$
(ii) $\mu=i-3 j+4 k, \gamma=4 i-j+3 k$
(iii) $\mu=\left[3 z-5\right], \gamma[6,-2]$
(iv) $\mu=\left[2,3,1\right], \gamma[2,4,1]$
2. Calculate the projection of $\underline{a}$ along $\underline{b}$ and projection of $\underline{b}$ along $\underline{a}$ when:
(i) $\quad a=i \quad k \neq b \quad j \quad k$
(ii) $\underline{a}=3 i+j-k, \underline{b}=-2 i-j+k$
3. Find a real number $\alpha$ so that the vectors $\mu$ and $\gamma$ are perpendicular.
(i) $\mu=2 \alpha i+j-k, \quad \gamma=i+\alpha j+4 k$
(ii) $\mu=\alpha i+2 \alpha j+3 k, \quad \gamma=i+\alpha j+3 k$
4. Find the number $z$ so that the triangle with vertices $A(1,-1,0), B(-2,2,1)$ and $C(0,2, z)$ is a right triangle with right angle at $C$.
5. If $\gamma$ is a vector for which
$\gamma_{i}=0, \gamma_{i j}=0, \gamma_{i} k=0$, find $\gamma_{i}$.
6. (i) Show that the vectors $3 i-2 j+k, i-3 j+5 k$ and $2 i+j-4 k$ form a right angle.
(ii) Show that the set of points $P=(1,3,2), Q=(4,1,4)$ and $P=(6,5,5)$ form a right triangle.
7. Show that mid point of hypotenuse a right triangle is equidistant from its vertices.
8. Prove that perpendicular bisectors of the sides of a triangle are concurrent.
9. Prove that the altitudes of a triangle are concurrent.
10. Prove that the angle in a semi circle is a right angle.
11. Prove that $\cos (\alpha+\beta)=\cos \alpha \cos \beta-\sin \alpha \sin \beta$
12. Prove that in any triangle $A B C$.
(i) $b=c \cos A+a \cos C$
(ii) $c=a \cos B+b \cos A$
(iii) $b^{2}=c^{2}+a^{2}-2 c a \cos B$
(iv) $c^{2}=a^{2}+b^{2}-2 a b \cos C$.