### 7.5.1 Analytical Expression of $\underline{u} \cdot(\underline{v} \times \underline{w})$

Let $\quad \underline{u}=a_{1} \underline{i}+b_{1} \underline{j}+c_{1} \underline{k}, \underline{v}=a_{2} \underline{i}+b_{2} \underline{j}+c_{2} \underline{k}$ and $\underline{w}=a_{3} \underline{i}+b_{3} \underline{j}+c_{3} \underline{k}$
Now $\quad \underline{v} \times \underline{w}=\left|\begin{array}{ccc}\underline{i} & \underline{j} & \underline{k} \\ a_{2} & b_{2} & c_{2} \\ a_{3} & b_{3} & c_{3}\end{array}\right|$

$$
\begin{aligned}
& \Rightarrow \quad \gamma \times \psi=\left(b_{1} c_{1}-b_{1} c_{2}\right) \xi-\left(a_{1} c_{1}-a_{1} c_{2}\right) \int+\left(a_{1} b_{1}-a_{1} b_{2}\right) \xi \\
& \therefore \quad \underline{u}_{1}(\gamma \times \psi)=a_{1}\left(b_{1} c_{1}-b_{1} c_{2}\right)-b_{1}\left(a_{1} c_{1}-a_{1} c_{2}\right)+c_{1}\left(a_{1} b_{1}-a_{1} b_{2}\right) \\
& \Rightarrow \quad \underline{u}_{1}(\gamma \times \psi)=\left|\begin{array}{ccc}
a_{1} & b_{1} & c_{1} \\
a_{2} & b_{2} & c_{2} \\
a_{1} & b_{1} & c_{1}
\end{array}\right| \\
& \text { which is called the determinant formula for scalar triple product of } u, \gamma \text { and } \psi \text { in } \\
& \text { component form. }
\end{aligned}
$$

$$
\begin{aligned}
& \text { Now } \quad \underline{u}_{1}(\gamma \times \psi)=\left|\begin{array}{ccc}
a_{1} & b_{1} & c_{1} \\
a_{2} & b_{2} & c_{2} \\
a_{3} & b_{3} & c_{3}
\end{array}\right| \\
& =-\left|\begin{array}{ccc}
a_{1} & b_{1} & c_{1} \\
a_{2} & b_{2} & c_{2} \\
a_{1} & b_{1} & c_{1}
\end{array}\right| \text { Interchanging } R_{1} \text { and } R_{2} \\
& =\left|\begin{array}{lll}
a_{2} & b_{2} & c_{2} \\
a_{3} & b_{3} & c_{3}
\end{array}\right| \text { Interchanging } R_{1} \text { and } R_{3} \\
& =\left|\begin{array}{lll}
a_{1} & b_{1} & c_{1}
\end{array}\right| \text { Interchanging } R_{2} \text { and } R_{3} \\
& =\left|\begin{array}{lll}
a_{2} & b_{2} & c_{2} \\
a_{3} & b_{3} & c_{3}
\end{array}\right| \text { Interchanging } R_{2} \text { and } R_{3} \\
& \text { ã„·. } \quad \underline{v}_{1}(\psi \times \underline{u})=\underline{v}_{2}(\underline{u} \times \underline{v}) \\
& \text { Hence } \quad \underline{u}_{1}(\gamma \times \psi)=\underline{v}_{2}(\gamma \times \underline{u})=\underline{v}_{2}(\gamma \times \gamma)
\end{aligned}
$$

Note:
(i) The value of the triple scalar product depends upon the cycle order of the vectors, but is independent of the position of the dot and cross. So the dot and cross, may be interchanged without altering the value i.e;
(ii) $(\underline{u} \times \underline{v}) \cdot \underline{w}=\underline{w} \cdot(\gamma \times \psi)=[\underline{u} \quad \underline{v} \quad \underline{w}]$
$(\gamma \times \psi) \cdot \underline{u}=\underline{v} \cdot(\psi \times \underline{u})=[\underline{v} \quad \underline{w} \quad \underline{u}]$
$(\psi \times \underline{u}) \cdot \underline{v}=\underline{w} \cdot(\underline{u} \times \underline{v})=[\underline{w} \quad \underline{u} \quad \underline{v}]$
(iii) The value of the product changes if the order is non-cyclic.
(iv) $\quad \underline{u}, \gamma, \psi$ and $\underline{u} \times(\gamma, \psi)$ are meaningless.