### 1.2.11 Odd Function

A function $f$ is said to be odd if $f(-x)=-f(x)$, for every number $x$ in the domain of $f$. For example, $\quad f(x)=x^{2}$ and $f(x)=\sin x$ are odd functions of $x$. Here

$$
f(-x)=(-x)^{2}=-x^{2}=-f(x) \text { and } f(-x)=\sin (-x)=-\sin x=-f(x)
$$

## Note: In both the cases, for each $x$ in the domain of $f,-x$ must also be in the domain of $f$

Example 1: Show that the parametric equations $x=a \cos t$ and $y=a \sin t$ represent the equation of the circle $x^{2}+y^{2}=a^{2}$

Solution: The parametric equations are

$$
\begin{aligned}
x=a \cos t & \text { (i) } \\
y=a \sin t & \text { (ii) }
\end{aligned}
$$

We eliminate the parameter " $t$ " from equations (i) and (ii).
By squaring we get, $\quad x^{2}=a^{2} \cos ^{2} t$

$$
y^{2}=a^{2} \sin ^{2} t
$$

By adding we get, $\quad x^{2}+y^{2}=a^{2} \cos ^{2} t+a^{2} \sin ^{2} t$

$$
=a^{2}\left(\cos ^{2} t+\sin ^{2} t\right)
$$

$\therefore x^{2}+y^{2}=a^{2}$, which is equation of the circle.
Example 2: $\quad$ Prove the identities
(i) $\cosh ^{2} x-\sinh ^{2} x=1$
(ii) $\cosh ^{2} x+\sinh ^{2} x=\cosh 2 x$

Solution: We know that $\sinh x=\frac{e^{x}-e^{-x}}{2}$

$$
\text { and } \quad \cosh x=\frac{e^{x}+e^{-x}}{2}
$$

Squaring (1) and (2) we have

$$
\begin{aligned}
& \sinh ^{2} x=\frac{e^{2 x}+e^{-2 x}-2}{4} \text { and } \cosh ^{2} x=\frac{e^{2 x}+e^{-2 x}+2}{4} \\
& \text { Now (i) } \quad \cosh ^{2} x-\sinh ^{2} x=\frac{e^{2 x}+e^{-2 x}+2}{4}-\frac{e^{2 x}+e^{-2 x}-2}{4} \\
& =\frac{e^{2 x}+e^{-2 x}+2-e^{2 x}-e^{-2 x}+2}{4}=\frac{4}{4} \\
& \therefore \quad \cosh ^{2} x-\sinh ^{2} x=1
\end{aligned}
$$

and (ii) $\cosh ^{2} x+\sinh ^{2} x=\frac{e^{2 x}+e^{-2 x}+2}{4}+\frac{e^{2 x}+e^{-2 x}-2}{4}$

$$
\begin{aligned}
& =\frac{e^{2 x}+e^{-2 x}+2+e^{2 x}+e^{-2 x}-2}{4} \\
& =\frac{2 e^{2 x}+2 e^{-2 x}}{4}=\frac{e^{2 x}+e^{-2 x}}{2} \\
\therefore \cosh ^{2} x+\sinh ^{2} x & =\cosh 2 x
\end{aligned}
$$

Example 3: Determine whether the following functions are even or odd.
(a) $f(x)=3 x^{4}-2 x^{2}+7$
(b) $f(x)=\frac{3 x}{x^{2}+1}$
(c) $f(x)=\sin x+\cos x$

## Solution:

(a) $f(-x)=3(-x)^{4}-2(-x)^{2}+7=3 x^{4}-2 x^{2}+7=f(x)$

Thus $\quad f(x)=3 x^{4}-2 x^{2}+7$ is even.
(b) $\quad f(-x)=\frac{3(-x)}{(-x)^{2}+1}-\frac{3 x}{x^{2}+1}=-f(x)$

Thus $\quad f(x)=\frac{3 x}{x^{2}+1}$ is odd
(c) $\quad f(-x)=\sin (-x)+\cos (-x)=-\sin x+\cos x \neq \pm f(x)$

Thus $f(x)=\sin x+\cos x$ is neither even nor odd

## EXERCISE 1.1

1. Given that:
(a) $f(x)=x^{2}-x$
(b) $f(x)=\sqrt{x+4}$

Find
(i) $f(-2)$
(ii) $f(0)$
(iii) $f(x-1)$
(iv) $f\left(x^{2}+4\right)$
2. Find $\frac{f(a+h)-f(a)}{h}$ and simplify where,
(i) $f(x)=6 x-9$
(ii) $f(x)=\sin x$
(iii) $f(x)=x^{3}+2 x^{2}-1$
(iv) $f(x)=\cos x$
3. Express the following:
(a) The perimeter $P$ of square as a function of its area $A$.
(b) The area $A$ of a circle as a function of its circumference $C$.
(c) The volume $V$ of a cube as a function of the area $A$ of its base.
4. Find the domain and the range of the function $g$ defined below, and
(i) $g(x)=2 x-5$
(ii) $g(x)=\sqrt{x^{2}-4}$
(iii) $g(x)=\sqrt{x+1}$
(iv) $g(x)=|x-3|$
(v) $g(x)=\left\{\begin{array}{lll}6 x+7 & , & x \leq-2 \\ 4-3 x & , & -2<x\end{array}\right.$
(vi) $g(x)=\left\{\begin{array}{lll}x-1 & , & x<3 \\ 2 x+1 & , & 3 \leq x\end{array}\right.$
(vii) $g(x)=\frac{x^{3}-3 x+2}{x+1}, x \neq-1$
(viii) $g(x)=\frac{x^{3}-16}{x-4}, x \neq 4$
5. Given $f(x)=x^{3}-a x^{2}+b x+1$

If $f(2)=-3$ and $f(-1)=0$. Find the values of $a$ and $b$.
6. A stone falls from a height of 60 m on the ground, the height $h$ after $x$ seconds is approximately given by $h(x)=40-10 x^{2}$
(i) What is the height of the stone when:.
(a) $x=1 \mathrm{sec}$ ?
(b) $x=1.5 \mathrm{sec}$ ?
(c) $x=1.7 \mathrm{sec}$ ?
(ii) When does the stone strike the ground?
7. Show that the parametric equations:
(i) $x=a t^{2}, y=2 a t$ represent the equation of parabola $y^{2}=4 a x$
(ii) $x=a \cos \theta, y=b \sin \theta$ represent the equation of ellipse $\frac{x^{2}}{a^{2}}+\frac{y^{2}}{b^{2}}=1$
(iii) $x=a \sec \theta, y=b \tan \theta$ represent the equation of hyperbola $\frac{x^{2}}{a^{2}}-\frac{y^{2}}{b^{2}}=1$
8. Prove the identities:
(i) $\sinh 2 x=2 \sinh x \cosh x$
(ii) $\operatorname{sech}^{2} x=1-\tanh ^{2} x$
(iii) $\operatorname{csch}^{2} x=\operatorname{coth}^{2} x-1$

9. Determine whether the given function *f* is even or odd.
   - (i) *f*(*x*) = *x*^2 + *x* (ii) *f*(*x*) = (*x* + 2)^2
   - (iii) *f*(*x*) = *x*√*x*^2 + 5 (iv) *f*(*x*) = *x* − 1/*x* + 1, *x* ≠ -1
   - (v) *f*(*x*) = *x*^2 + 6 (vi) *f*(*x*) = *x*^2 − *x*/*x* + 1

# **1.3 COMPOSITION OF FUNCTIONS AND INVERSE OF AFUNCTION**

Let *f* be a function from set *X* to set *Y* and *g* be a function from set *Y* to set *Z*. The composition of *f* and *g* is a function, denoted by *gof*, from *X* to *Z* and is defined by

(*gof*(*x*) = *g*(*f*(*x*)) = *gf*(*x*), for all *x* ∈ *X*).