#### **Explanation**

Consider two real valued functions *f* and *g* defined by

*f*(*x*) = 2*x* + 3 and *g*(*x*) = *x*^2

then *gof*(*x*) = *g*(*f*(*x*)) = *g*(2*x* + 3) = (2*x* + 3)^2

The arrow diagram of two successive mappings, *f*, *g*, is denoted by *gf* and is shown in the figure.

Thus a single composite function *gf*(*x*) is equivalent to two successive functions *f* followed by *g*.

**Example 1:** Let the real valued functions *f* and *g* be defined by

*f*(*x*) = 2*x* + 1 and *g*(*x*) = *x*^2 âˆ’ 1

Obtain the expressions for (i) *fg* (*x*) (ii) *gf*(*x*) (iii) *f*^2 (*x*) (iv) *g*^2 (*x*)