### 2.5 DERIVATIVES OF INVERSE FUNCTIONS

If for each $x \in \mathrm{D}_{t}, f(x)=y$ and for each $y \in \mathrm{D}_{g}, g(x)=x$, then $f$ and $g$ are inverse of each other, that is,

$$
(g \text { of })(x)=g(f(x))=g(y)=x
$$

and $(f \text { o g })(y)=f(g(y))=f(x)=y$
Using chain rule, we can prove that

$$
f^{\prime}(x) \cdot g^{\prime}(y)=1
$$

$\Rightarrow f^{\prime}(x)=\frac{1}{g^{\prime}(y)}$
$\Rightarrow \frac{d y}{d x}=\frac{1}{\frac{d x}{d y}} \quad\left(\begin{array}{l}\cdot \cdot \quad f(x)=y \Rightarrow f^{\prime}(x)=\frac{d y}{d x} \\ \text { and } g(y)=x \Rightarrow g^{\prime}(y)=\frac{d x}{d y}\end{array}\right)$