#### 4.1.1 The Distance Formula

Let *A* (*x*<sub>1</sub>, *y*<sub>1</sub>) and *B* (*x*<sub>2</sub>, *y*<sub>2</sub>) be two points in the plane. We can find the distance *d* = |*AB*| from the right triangle *AQB* by using the Pythagorean theorem. We have

$$
d = AB = AQ + QB^2 \tag{1}
$$

|*AQ*| = |*BS*| = |*BO* + *OS*|

|*OR* | *OS*|

|*SB*| = |*SB* - *SQ*|

|*y*<sub>1</sub> | *y*<sub>1</sub> | | || || | | | | | | | | | | | | | | | | | | | | | | | | | | | | | | | | | | | | | | | | | | | | | | | | | | | | | | | | | | | | | | | | | | | | | | | | | | | | | | | | | | | | | | | | | | | | | | | | | | | | | | | | | | | | | | | | | | | | | | | | | | | | | | | | | | | | | | | | | | | | | | | | | | | | | | | | | | | | | | | | | | | | | | | | | | | | | | | | | | | | | | | | | | | | | | | | | | | | | | | | |

or

$$
x = \frac{k_1 v_1 + k_2 v_2}{k_1 + k_2}
$$

Similarly, by drawing perpendiculars from *A*, *B* and *P* to the *y*-axis and proceeding as before, we can show that

$$
y = \frac{k_1 v_1 + k_2 v_2}{k_1 + k_2}
$$