### 4.3.6 To Transform the General Linear Equation to Standard Forms

Theorem: To transform the equation $a x+b y+c=0$ in the standard form

## 1. Slope-Intercept Form.

We have

$$
b y=-a x-c \quad \text { or } \quad y=\frac{-a}{b} \times-\frac{c}{b}=m x+c \text {, where } m=\frac{-a}{b}, c=\frac{-c}{b}
$$

## 2. Point - Slope Form

We note from (1) above that slope of the line $a x+b y+c=0$ is $\frac{-a}{b}$. A point on the line is $\left(\frac{-c}{a}, 0\right)$

Equation of the line becomes $y=\frac{-a}{b}\left(x+\frac{c}{a}\right)$
which is in the point-slope form.

## 3. Symmetric Form

$$
m=\tan \alpha=\frac{-a}{b} \cdot \sin \alpha=\frac{a}{\pm \sqrt{a^{2}+b^{2}}} \cdot \cos \alpha \quad \frac{b}{\pm \sqrt{a^{2}+b^{2}}}
$$

A point on $a x+b y+c=0$ is $\left(\frac{-c}{a}, 0\right)$
Equation in the symmetric form becomes

$$
\frac{x-\left(-\frac{c}{a}\right)}{b / \pm \sqrt{a^{2}+b^{2}}}=\frac{y-0}{a / \pm \sqrt{a^{2}+b^{2}}} \quad r
$$

is the required transformed equation. Sign of the radical to be properly chosen.

## 4. Two -Point Form

We choose two arbitrary points on $a x+b y+c=0$. Two such points are $\left(\frac{-c}{a}, 0\right)$ and $\left(0, \frac{-c}{b}\right)$. Equation of the line through these points is

$$
\frac{y-0}{0+\frac{c}{b}}=\frac{x+\frac{c}{a}}{-\frac{c}{a}-0} \quad \text { i.e., } y \quad 0 \quad \frac{-a}{b}\left(x \quad \frac{c}{a}\right)
$$

## 5. Intercept Form.

$$
a x+b y=-c \quad \text { or } \quad \frac{a x}{-c}+\frac{b y}{-c}=1 \quad \text { i.e } \quad \frac{x}{-c / a} \quad \frac{y}{-c / b} \quad 1=
$$

which is an equation in two intercepts form.

## 6. Normal Form.

The equation: $a x+b y+c=0$
can be written in the normal form as:

$$
\frac{a x+b y}{\pm \sqrt{a^{2}+b^{2}}}=\frac{-c}{\pm \sqrt{a^{2}+b^{2}}}
$$

The sign of the radical to be such that the right hand side of (2) is positive.
Proof. We know that an equation of a line in normal form is

$$
x \cos \alpha+y \sin \alpha=p
$$

If (1) and (3) are identical, we must have

$$
\frac{a}{\cos \alpha}=\frac{b}{\sin \alpha}=\frac{-c}{p}
$$

i.e.,

$$
\frac{p}{-c}=\frac{\cos \alpha}{a}=\frac{\sin \alpha}{b}=\frac{\sqrt{\cos ^{2} \alpha+\sin ^{2} \alpha}}{\pm \sqrt{a^{2}+b^{2}}} \quad \frac{1}{\pm \sqrt{a^{2}+b^{2}}}
$$

Hence, $\quad \cos \alpha=\frac{a}{\pm \sqrt{a^{2}+b^{2}}}$ and $\sin \alpha \quad \frac{b}{\pm \sqrt{a^{2}+b^{2}}}$
Substituting for $\cos \alpha, \sin \alpha$ and $p$ into (3), we have

$$
\frac{a x+b y}{\pm \sqrt{a^{2}+b^{2}}}=\frac{-c}{\pm \sqrt{a^{2}+b^{2}}}
$$

Thus (1) can be reduced to the form (2) by dividing it by $\pm \sqrt{a^{2}+b^{2}}$. The sign of the radical to be chosen so that the right hand side of (2) is positive.

Example 1: Transform the equation $5 x-12 y+39=0$ into
(i) Slope intercept form.
(ii) Two-intercept form.
(iii) Normal form.
(iv) Point-slope form.
(v) Two-point form.
(vi) Symmetric form.

## Solution:

(i) We have $12 y=8 x \quad 39$ or $=y \quad \frac{5}{12} x \quad \frac{39}{12} y m \quad \frac{5}{12}, y$-intercept $c=\frac{39}{12}$
(ii) $5 x-12 y=39$ or $\frac{5 x}{-39} \quad \frac{12 y}{39} \quad 1$ or $\frac{x}{-39 / 5} \quad \frac{y}{39 / 12} \quad 1$ is the required equation.
(iii) $5 x-12 y=39$. Divide both sides by $\pm \sqrt{5^{2}+125}=13$. Since R.H.S is to be positive, we have to take negative sign.

Hence $=\frac{5 x}{-13}+\frac{12 y}{13}=3$ is the normal form of the equation.
(iv) A point on the line is $\left(\frac{-39}{5}, 0\right)$ and its slope is $\frac{5}{12}$.

Equation can be written as: $y-0=\frac{5}{12}\left(x+\frac{39}{5}\right)$
(v) Another point on the line is $\left(0, \frac{39}{12}\right)$. Line through $\left(\frac{-39}{5}, 0\right)$ and $\left(0, \frac{39}{12}\right)$ is

$$
\frac{y-0}{0-\frac{39}{12}}=\frac{x+\frac{39}{5}}{-\frac{39}{5}-0}
$$

(vi) We have $\tan \alpha=\frac{5}{12}=m, \sin \alpha=\frac{5}{13}, \cos \alpha=\frac{12}{13}$. A point of the line is $\left(\frac{-39}{5}, 0\right)$. Equation of the line in symmetric form is

$$
\frac{x+39 / 5}{12 / 13}=\frac{y-0}{5 / 13}=r(\text { say })
$$

Example 2: $\quad$ Sketch the line
$3 x+2 y+6=0$.

Solution: To sketch the graph of (1), we find two points on it. If $y=0, x=-2$ and if $x=0, y=-3$.

Thus $x$ intercept $=-2$
$y$ intercept $=-3$
The points $A(-2,0), B(0,-3)$ are on (1). Plot these points in the plane and draw the straight line through $A$ and $B$. It is the graph of (1).

Example 3: $\quad$ Find the distance between the parallel lines
$2 x+y+2=0$
and $\quad 6 x+3 y-8=0$
(1)

Sketch the lines. Also find an equation of the line parallel to the given lines and lying midway between them.

Solution: We first convert both the lines into normal form. (1) can be written as $2 x+y=-2$
Dividing both sides by $-\sqrt{4+1}$, we have

$$
\frac{-2}{\sqrt{5}} x+\frac{-y}{\sqrt{5}}=\frac{2}{\sqrt{5}}
$$

which is normal form of (1). Normal form of (2) is

$$
\frac{6 x}{\sqrt{45}}+\frac{3 y}{\sqrt{45}}=\frac{8}{\sqrt{45}}
$$

i.e., $\frac{2 x}{\sqrt{5}}+\frac{y}{\sqrt{5}}=\frac{8}{3 \sqrt{5}}$

Length of the perpendicular from $(0,0)$ to the line (1) is $\frac{-}{\sqrt{5}}[$ From (3)]
Similarly, length of the perpendicular from $(0,0)$ to the line (2) is $\frac{8}{3 \sqrt{5}}$ [From (4)]

From the graphs of the lines it is clear that the lines are on opposite sides of the origin, so the distance between them equals the sum of the two perpendicular lengths.
i.e., Required distance $=\frac{2}{\sqrt{5}}+\frac{8}{3 \sqrt{5}}=\frac{14}{3 \sqrt{5}}$

The line parallel to the given lines lying midway between them is such that length of the perpendicular
from $O$ to the line $=\frac{8}{3 \sqrt{5}}-\frac{7}{3 \sqrt{5}}\left(\right.$ or $\frac{7}{3 \sqrt{5}}-\frac{2}{\sqrt{5}}$ ) $=\frac{1}{3 \sqrt{5}}$
Required line is $=\frac{2 x}{\sqrt{5}}+\frac{y}{\sqrt{5}}=-\frac{1}{3 \sqrt{5}}$ or $6 x+3 y=1$