### 4.6.1 Homogeneous Equation

Let $f(x, y)=0$
be any equation in the variables $x$ and $y$. Equation (1) is called a homogeneous equation of degree $n$ (a positive integer) if

$$
f(k x, k y)=k^{n} f(x, y)
$$

for some real number $k$.
For example, in equation (5) above if we replace $x$ and $y$ by $k x$ and $k y$ respectively, we have

$$
\begin{aligned}
& k^{2} y^{2}-k^{2}\left(m_{1}+m_{2}\right) x y+k^{2} m_{1} m_{2} x^{2}=0 \\
\text { or } & k^{2}\left[y^{2}-\left(m_{1}+m_{2}\right) x y+m_{1} m_{2} x^{2}\right]=0 \quad \text { i.e., } \quad k^{2} f(x, y) \quad 0
\end{aligned}
$$

Thus (5) is a homogeneous equation of degree 2.

$$
a x^{2}+2 h x y+b y^{2}=0
$$

A general second degree homogeneous equation can be written as:

$$
a x^{2}+2 h x y+b y^{2}=0
$$

provided $a, h$ and $b$ are not simultaneously zero.

Theorem: Every homogenous second degree equation

$$
a x^{2}+2 h x y+b y^{2}=0
$$

represents a pair of lines through the origin. The lines are
(i) real and distinct, if $h^{2}>a b$
(ii) real and coincident, if $h \quad a b$
(iii) imaginary, if $h^{2}<a b$

Proof: Multiplying (1) by b and re-arranging the terms, we have

$$
b^{2} y^{2}+2 b k x y+a b x^{2}=0
$$

or $\quad b^{2} y^{2}+2 b k x y+h^{3} x^{2}-h^{3} x^{2}+a b x^{2}=0$
or $\quad(b y+h x)^{3}-x^{2}\left(h^{3}-a b\right)=0$
or $\quad(b y+h x+x \sqrt{h^{3}-a b})(b y+h x-x \sqrt{h^{3}-a b})=0$
Thus (1) represents a pair of lines whose equations are:

$$
b y+x\left(h+\sqrt{h^{3}-a b}\right)=0
$$

and $b y+x\left(h-\sqrt{h^{3}-a b}\right)=0$
Clearly, the lines (2) and (3) are
(i) real and distinct if $h^{3}>a b$. (ii) real and coincident, if $h^{3}=a b$.
(iii) imaginary, if $h^{3}<a b$.

It is interesting to note that even in case the lines are imaginary, they intersect in a real point viz $(0,0)$ since this point lies on their joint equation (1).

Example: Find an equation of each of the lines represented by

$$
20 x^{2}+17 x y-24 y^{2}=0
$$

Solution. The equation may be written as

$$
\begin{aligned}
& 24\left(\frac{y}{x}\right)^{2}-17\left(\frac{y}{x}\right)-20=0 \\
& \Rightarrow \quad \frac{y}{x}=\frac{17 \pm \sqrt{289+1920}}{48}-\frac{17 \pm 47}{48}-\frac{4}{3}-\frac{-5}{8} \\
& \Rightarrow \quad y=\frac{4}{3} x \quad \text { and } \quad y=\frac{-5}{8} x \\
& \Rightarrow \quad 4 x-3 y=0 \quad \text { and } \quad 5 x+8 y=0
\end{aligned}
$$

version: 1.1