### 6.9.2 n Harmonic Means between two Numbers

$H_{1}, H_{2}, H_{3}, \cdots, H_{n}$ are called $n$ harmonic means (H.Ms.) between $a$ and $b$ if $a, H_{1}, H_{2}, H_{3}, \cdots, H_{n}, b$ are in H.P. If we want to insert $n$ H.Ms., between $a$ and $b$, we first find $n$ A.Ms. $A_{1}, A_{2}, \ldots, A_{n}$ between $\frac{1}{a}$ and $\frac{1}{b}$, then take their reciprocals to get $n$ H.Ms. between $a$ and $b$, that is, $\frac{1}{A_{1}}, \frac{1}{A_{2}}, \cdots, \frac{1}{A_{n}}$ will be the required $n$ H.Ms. between $a$ and $b$.
Example 24 Find three harmonic means between $\frac{1}{5}$ and $\frac{1}{17}$.
Solution Let $A_{1}, A_{2}, A_{3}$ be three A.Ms. between 5 and 17, that is,

$$
5, A_{1}, A_{2}, A_{3}, 17 \text { are in A.P. }
$$

Using $\quad a_{n}=a_{1}+(n-1) d$, we get

$$
\begin{aligned}
17 & =5+(5-1) d \\
4 d & =12 \\
\Rightarrow \quad d & =3
\end{aligned} \quad\left(\because a_{2}=17 \text { and } a_{1}=5\right)
$$

Thus, $\quad A_{1}=5+3=8, A_{2}=5+2(3)=11$ and $A_{3}=5+3(3)=14$
Hence $\frac{1}{8}, \frac{1}{11}, \frac{1}{14}$ are the required harmonic means.

# EXERCISE 6.9

1. Find the $9^{\text {th }}$ term of the following harmonic sequences:
(i) $\frac{1}{3}, \frac{1}{5}, \frac{1}{7}, \ldots$
(ii) $\frac{-1}{5}, \frac{-1}{3},-1, \ldots$
2. Insert five harmonic means between the following given numbers:
(i) $\frac{-2}{5}$ and $\frac{2}{13}$
(ii) $\frac{1}{4}$ and $\frac{1}{24}$
3. The first term of an H.P. is $-\frac{1}{3}$ and the fifth term is $\frac{1}{5}$. Find its $9^{\text {th }}$ term.
4. If 5 is the harmonic mean between 2 and $b$, find $b$.
5. If the numbers $\frac{1}{k}, \frac{1}{2 k+1}$ and $\frac{1}{4 k-1}$ are in harmonic sequence, find $k$.
6. Find $n$ so that $a^{n+1}+b^{n+1}$ may be H.M. between $a$ and $b$.
7. If $a^{2}, b^{2}$ and $c^{2}$ are in A.P., show that $a+b, c+a$ and $b+c$ are in H.P.
8. If the H.M. and A.M. between two numbers are 4 and $\frac{9}{2}$ respectively, find the numbers.
9. If the (positive) G.M. and H.M. between two numbers are 4 and $\frac{16}{5}$, find the numbers.
10. If $\frac{b+c-a}{a} \frac{c+a-b}{b}, \frac{a+b-c}{c}$ are in A.P., show that $a, b, c$ are in H.P.

11. If $a, b, c, d$ are in H.P., show that $3(a-b)(c-d)=(b-c)(a-d)$.
12. If between any two numbers there are inserted two A.Ms. $A_{1}, A_{2}$, two G.Ms. $G_{1}$, $G_{2}$ and two H.Ms. $H_{1}, H_{2}$; show that $\frac{A_{1}+A_{2}}{G_{1} G_{2}}=\frac{H_{1}+H_{2}}{H_{1} H_{2}}$.
13. The H.M. of two numbers is 4 . The A.M., $A$ and the G.M., $G$ satisfy the relation $2 A+G^{2}=27$. Find the numbers.
14. First three of the four numbers $a, b, c, d$ are in A.P., and the next three are in H.P., show that $a d=b c$.
15. If $a, b, c$ are in G.P., show that $\log _{a} x, \log _{b} x, \log _{c} x$ are in H.P.
16. If $a, b, c$ are in H.P., show that
(i) $\frac{a-b}{b-c}=\frac{a}{c}$
(ii) $(a-c)^{2}=(a+c)\left(a-2 b+c\right)$.
17. If $2+x, 5+x$ and $9+x$ are in H.P., find the value of $x$.
18. If the roots of the equation $a(b-c) x^{2}+b(c-a) x+c(a-b)=0$ are equal, prove that $a, b, c$ are in H.P.

# 6.10 Miscellaneous Series

The Greek letter $\Sigma$ (sigma) is used to denote sums of different types. For example, the notation $\sum_{i=m}^{n} a_{i}$ is used to express the $\operatorname{sum} a_{m}+a_{m+1}+a_{m+2}+\cdots+a_{n}$ and the sum expression $1+3+5+\cdots$ to $n$ terms is written as $\sum_{k=1}^{n}(2 k-1)$, where $2 k-1$ is the $k^{\text {th }}$ term of the sum and $k$ is called the index of summation. 1 and $n$ are called the lower limit and upper limit of summation respectively.
The sum of the first $n$ natural numbers, the sum of squares of the first $n$ natural numbers and the sum of the cubes of the first $n$ natural numbers are expressed in sigma notation as:

$$
1+2+3+\cdots+n=\sum_{k=1}^{n} k ; 1^{2}+2^{2}+3^{2}+\cdots+n^{2}=\sum_{k=1}^{n} k^{2} ; 1^{3}+2^{3}+3^{3}+\cdots+n^{3}=\sum_{k=1}^{n} k^{3}
$$

We evaluate $\sum_{k=1}^{n}\left[k^{m}-(k-1)^{m}\right]$ for any positive integer $m$ and we shall use this result to find out formulae for three expressions stated above.

$$
\begin{aligned}
\sum_{k=1}^{n}\left[k^{m}-(k-1)^{m}\right]=\left(1^{m}-0^{m}\right)+\left(2^{m}-1^{m}\right)+\left(3^{m}-2^{m}\right)+ & \cdots \\
& +\left[(n-1)^{m}-(n-2)^{m}\right]+\left[n^{m}-(n-1)^{m}\right]=n^{m}
\end{aligned}
$$

i.e., $\quad \sum_{k=1}^{n}\left[\left(k^{m}-(k-1)^{m}\right]=n^{m}\right.$
If $m=1$, then $\sum_{k=1}^{n}\left[\left(k^{1}-(k-1)^{1}\right]=n^{1}\right.$ i.e., $\sum_{k=1}^{n} 1=n$
If $m=2$, then $\sum_{k=1}^{n}\left[k^{2}-(k-1)^{2}\right]=n^{2}$

## Properties of Summation:

(i) $\sum_{s=1}^{n}\left(a_{s}+b_{s}\right)=\sum_{s=1}^{n} a_{s}+\sum_{s=1}^{n} b_{s}$
(ii) $\sum_{s=1}^{n} \alpha a_{s}=\alpha \sum_{s=1}^{n} a_{s}$

To Find the Formulae for the Sums
(i) $\sum_{k=1}^{n} k$
(ii) $\sum_{k=1}^{n} k^{2}$
(iii) $\sum_{k=1}^{n} k^{3}$
(i) We know that $(k-1)^{2}=k^{2}-2 k+1$ and this identity can be written as:

$$
k^{2}-(k-1)^{2}=2 k-1
$$

Taking summation on both sides of (A) from $k=1$ to $n$, we have

$$
\begin{aligned}
& \sum_{k=1}^{n}\left[\left(k^{2}-(k-1)^{2}\right]=\sum_{k=1}^{n}(2 k-1)\right. \\
& \text { i.e., } \\
& n^{2}=2 \sum_{k=1}^{n} k-n \\
& \text { or } \\
& 2 \sum_{k=1}^{n} k=n^{2}+n \\
& \text { Thus }
\end{aligned}
$$

$$
\sum_{k=1}^{n} k=\frac{n(n+1)}{2}
$$

Similarly, we can prove easily
(ii) $\sum_{k=1}^{n} k^{2}=\frac{n(n+1)(2 n+1)}{6}$
(iii) $\sum_{k=1}^{n} k^{3}=\left[\frac{n(n+1)}{2}\right]^{2}$

Example 25 Find the sum of the series $1^{3}+3^{3}+5^{3}+\ldots$ to $n$ terms.
Solution $T_{k}=(2 k-1)^{2} \quad(\because 1+2(k-1)=2 k-1)$

$$
=8 k^{3}-12 k^{2}+6 k-1
$$

Let $S_{n}$ denote the sum of $n$ terms of the given series, then

$$
S_{n}=\sum_{k=1}^{n} T_{k}
$$

or

$$
S_{n}=\sum_{k=1}^{n}\left(8 k^{3}-12 k^{2}+6 k-1\right)
$$

$$
\begin{aligned}
& =8 \sum_{k=1}^{n} k^{3}-12 \sum_{k=1}^{n} k^{2}+6 \sum_{k=1}^{n} k-\sum_{k=1}^{n} 1 \\
& =8\left[\frac{n(n+1)}{2}\right]^{2}-12\left[\frac{n(n+1)(2 n+1)}{6}\right]+6\left[\frac{n(n+1)}{2}\right]-n \\
& =2 n^{2}(n+1)^{2}-2 n(n+1)(2 n+1)+3 n(n+1)-n \\
& =2 n^{2}\left(n^{2}+2 n+1\right)-2 n\left(2 n^{2}+3 n+1\right)+n(3 n+3)-n \\
& =2 n\left[\left(n^{3}+2 n^{2}+n\right)-\left(2 n^{2}+3 n+1\right)\right]+n(3 n+3-1) \\
& =2 n\left(n^{3}-2 n-1\right)+n(3 n+2) \\
& =2 n\left(n^{3}-2 n-1\right)+n(3 n+2) \\
& =n\left[2 n^{3}-4 n-2+3 n+2\right] \\
& =n\left[2 n^{3}-n\right]=n\left[n\left(2 n^{2}-1\right)\right] \\
& =n^{2}\left[2 n^{2}-1\right]
\end{aligned}
$$

Example 26 Find the sum of $n$ terms of series whose $n^{\text {th }}$ terms is $n^{3}+\frac{3}{2} n^{2}+\frac{1}{2} n+1$.
Solution Given that

$$
T_{n}=n^{3}+\frac{3}{2} n^{2}+\frac{1}{2} n+1
$$

Thus

$$
T_{k}=k^{3}+\frac{3}{2} k^{2}+\frac{1}{2} k+1
$$

and

$$
5_{n}=\sum_{k=1}^{n}\left(k^{3}+\frac{3}{2} k^{2}+\frac{1}{2} k+1\right)
$$

$$
\begin{aligned}
& =\sum_{k=1}^{n} k^{3}+\frac{3}{2} \sum_{k=1}^{n} k^{2}+\frac{1}{2} \sum_{k=1}^{n} k+\sum_{k=1}^{n} 1 \\
& =\frac{n^{2}(n+1)^{2}}{4}+\frac{3}{2} \times \frac{n(n+1)(2 n+1)}{6}+\frac{1}{2} \times\left[\frac{n(n+1)}{2}\right]+n \\
& =\frac{n}{4}\left[n\left(n^{2}+2 n+1\right)+\left(2 n^{2}+3 n+1\right)+(n+1)+4\right] \\
& =\frac{n}{4}\left(n^{3}+2 n^{2}+n+2 n^{2}+3 n+1+n+1+4\right) \\
& =\frac{n}{4}\left(n^{3}+4 n^{2}+5 n+6\right)
\end{aligned}
$$

# EXERCISE 6.10

1. Sum the following series upto $n$ terms.
(i) $1 \times 3+2 \times 5+3 \times 7+\cdots$
(ii) $1 \times 5+2 \times 8+3 \times 11+\cdots$
(iii) $1 \times 2+2 \times 5+3 \times 8+\cdots$
(iv) $1 \times 3 \times 5+2 \times 4 \times 6+3 \times 5 \times 7+\cdots$
(v) $1 \times 2 \times 4+2 \times 3 \times 7+3 \times 4 \times 10+\cdots$
(vi) $2^{2}+4^{2}+6^{2}+\cdots$
(vii) $3^{2}+6^{2}+9^{2}+\cdots$
(viii) $4 \times 1^{2}+7 \times 2^{2}+10 \times 3^{2}+\cdots$
(ix) $3+(3+7)+(3+7+11)+\cdots$
(x) $1^{2}+\left(1^{2}+2^{2}\right)+\left(1^{2}+2^{2}+3^{2}\right)+\cdots$
2. Sum the series.
(i) $1^{2}-2^{2}+3^{2}-4^{2}+\ldots+(2 n-1)^{2}-(2 n)^{2}$
(ii) $\frac{1^{2}}{1}+\frac{1^{2}+2^{2}}{2}+\frac{1^{2}+2^{2}+3^{2}}{3}+\ldots$ to $n$ terms :
3. Find the sum to $n$ terms of the series whose $n^{\text {th }}$ terms are given.
(i) $5 n^{2}+2 n+3$
(ii) $n^{2}+2 n-3$
4. Given $n^{\text {th }}$ terms of the series, find the sum to $2 n$ terms:
(i) $3 n^{2}+5 n+2$
(ii) $n^{2}+n-2$