### 6.1.1 General Form of an Equation of a Circle

Theorem: The equation

$$
x^{2}+y^{2}+2 g x+2 f y+c=0
$$

represents a circle $g, f$ and $c$ being constants.
Equation (1) can be written as:

$$
\left(x^{2}+2 g x+g^{2}\right)+\left(y^{2}+2 f y+f^{2}\right)=g^{2}+f^{2}-c
$$

or

$$
[x-(-g)]^{2}+\left[y-(-f)\right]^{2}=\left(\sqrt{g^{2}+f^{2}-c}\right)^{2}
$$

which is standard form of an equation of a circle with centre $(-g,-f)$ and radius $\sqrt{g^{2}+f^{2}-c}$.
The equation (1) is called general form of an equation of a circle.

## Note:

1. (1) is a second degree equation in which coefficient of each of $x^{2}$ and $y^{2}$ is 1 .
2. (1) contains no term involving the product $x y$.

Thus a second degree equation in which coefficients of $x^{2}$ and $y^{2}$ are equal and there is no product term $x y$ represents a circle.

If three non-collinear points through which a circle passes are known, then we can find the three constants $f, g$ and $c$ in (1).

Example 2: Show that the equation:

$$
5 x^{2}+5 y^{2}+24 x+36 y+10=0
$$

represents a circle. Also find its centre and radius.
Solution: The given equation can be written as:

$$
x^{2}+y^{2}+\frac{24}{5} x+\frac{36}{5} y+2=0
$$

which is an equation of a circle in the general form. Here

$$
g=\frac{12}{5} \cdot f=\frac{18}{5} \cdot c=2
$$

$$
\begin{aligned}
& \text { Thus centre of the circle }=(-g,-f)=\left(\frac{-12}{5}, \frac{-18}{5}\right) \\
& \text { Radius of the circle }=\sqrt{g^{2}+f^{2}-c}=\sqrt{\frac{144}{25}+\frac{324}{25}-2} \\
& =\sqrt{\frac{418}{25}}=\frac{\sqrt{418}}{5}
\end{aligned}
$$