### 6.7 TANGENTS AND NORMALS

We have already seen in the geometrical interpretation of the derivative of a curve $y=f(x)$ or $f(x, y)=0$ that $\frac{d y}{d x}$ represents the slope of the tangent line to the curve at the point $(x, y)$. In order to find an equation of the tangent to a given
conic at some point on the conic, we shall first find the slope of the tangent at the given point by calculating $\frac{d y}{d x}$ from the equation of the conic at that point and then using the point - slope form of a line, it will be quite simple to write an equation of the tangent. Since the normal to a curve at a point on the curve is perpendicular to the tangent through the point of tangency, its equation can be easily written.

Example 1. Find equations of the tangent and normal to
(i) $y^{2}=4 a x$
(ii) $\frac{x^{2}}{a^{2}}+\frac{y^{2}}{b^{2}}=1$
(iii) $\frac{x^{2}}{a^{2}}-\frac{y^{2}}{b^{2}}=1$
at the point $\left(x_{1}, y_{1}\right)$.
Solution: (i). Differentiating (1) w.r.t. $x$, we get

$$
\begin{aligned}
& 2 y \frac{d y}{d x}=4 a \quad \text { or } \quad \frac{d y}{d x} \quad 2 a \\
& \left.\frac{d y}{d x}\right|_{x_{1}, y_{1}}=\frac{2 a}{y_{1}} \text { Slope of the tangent at }\left(x_{1}, y_{1}\right)
\end{aligned}
$$

Equation of the tangent to (1) at $\left(x_{1}, y_{1}\right)$ is

$$
y-y_{1}=\frac{2 a}{y_{1}}\left(x-x_{1}\right) \text { or } y y_{1}-y_{1}^{2}=2 a x-2 a x_{1} \text { or } y y_{1}-2 a x=y_{1}^{2}-2 a x_{1}
$$

Adding $-2 a x$, to both sides of the above equation, we obtain

$$
y y_{1}=2 a\left(x+x_{1}\right)=y_{1}^{2}-4 a x_{1}
$$

Since $\left(x_{1}, y_{1}\right)$ lies on $y^{2}=4 a x_{1}$ so $y_{1}^{2}-4 a x_{1}=0$
Thus equation of the required tangent is

$$
y y_{1}=2 a\left(x+x_{1}\right)
$$

Slope of the normal $=\frac{-y_{1}}{2 a} \quad$ (negative reciprocal of slope of the tangent)

Equation of the normal is

$$
y-y_{1}=\frac{-y_{1}}{2 a}\left(x-x_{1}\right)
$$

(ii) $\frac{x^{2}}{a^{2}}+\frac{y^{2}}{b^{2}}=1$

Differentiating the above equation, w.r.t. $x$, we have

$$
\frac{2 x}{a^{2}}+\frac{2 y}{b^{2}} \frac{d y}{d x}=0-\text { or } \frac{d y}{d x}=\frac{b^{2} x}{a^{2} y}
$$

or $\left.\frac{d y}{d x}\right|_{\left(x_{1}, y_{1}\right)}=\frac{-b^{2} x_{1}}{a^{2} y_{1}}$
Equation of the tangent to (2), at $\left(x_{1}, y_{1}\right)$ is

$$
y-y_{1}=\frac{-b^{2} x_{1}}{a^{2} y_{1}}\left(x-x_{1}\right)
$$

or $\quad \frac{y y_{1}}{b^{2}}, \frac{y_{1}^{2}}{b^{2}}=\frac{-x x_{1}}{a^{2}}+\frac{x_{1}^{2}}{a^{2}} \quad$ or $\quad \frac{x x_{1}}{a^{2}}+\frac{y y_{1}}{b^{2}}=\frac{x^{2}}{a^{2}}+\frac{y_{1}^{2}}{a^{2}}$
Since $\left(x_{1}, y_{1}\right)$ lie on (2) so, $\frac{x_{1}^{2}}{a^{2}}+\frac{y_{1}^{2}}{b^{2}}=1$
Hence an equation of the tangent to (2) at $\left(x_{1}, y_{1}\right)$ is $\frac{x x_{1}}{a^{2}}+\frac{y y_{1}}{b^{2}}=1$
Slope of the normal at $\left(x_{1}, y_{1}\right)$ is $\frac{a^{2} y_{1}}{b^{2} x_{1}}$.
Equation of the normal at $\left(x_{1}, y_{1}\right)$ is

$$
y-y_{1}=\frac{a^{2} y_{1}}{b^{2} x_{1}}\left(x-x_{1}\right)
$$

or $\quad b^{2} x_{1} y-b^{2} x_{1} y_{1}=a^{2} y_{1} x-a^{2} x_{1} y_{1} \quad$ or $\quad a^{2} y_{1} x-b^{2} x_{1} y=x_{1} y_{1}\left(a^{2}-b^{2}\right)$
Dividing both sides of the above equation by $x_{1} y_{1}$, we get
$\frac{a^{2} x}{x_{1}} \quad \frac{b^{2} y}{y_{1}}=a^{2}-b^{2}$, as an equation of the normal.
(iii) Proceeding as in (ii), it is easy to see that equations of the tangent and normal to (3) at $\left(x_{1}, y_{1}\right)$ are

$$
\frac{x x_{1}}{a^{2}}+\frac{y y_{1}}{b^{2}}=1 \quad \text { and } \quad \frac{a^{2} x}{x_{1}}+\frac{b^{2} y}{y_{1}}=a^{2}+b^{2}, \text { respectively. }
$$

## Remarks

An equation of the tangent at the point $\left(x_{1}, y_{1}\right)$ of any conic can be written by making replacements in the equation of the conic as under:

$$
\begin{array}{lll}
\text { Replace } & x^{2} & \text { by } & x x_{1} \\
& y^{2} & \text { by } & y y_{1} \\
& x & \text { by } & \frac{1}{2}\left(x+x_{1}\right) \\
& y & \text { by } & \frac{1}{2}\left(y+y_{1}\right)
\end{array}
$$

Example 1. Write equations of the tangent and normal to the parabola $x^{2}=16 y$ at the point whose abscissa is 8 .

Solution: Since $x=8$ lies on the parabola, substituting this value of $x$ into the given equation, we find

$$
64=16 y \quad \text { or } \quad y=4
$$

Thus we have to find equations of tangent and normal at $(8,4)$.
Slope of the tangent to the parabola at $(8,4)$ is 1 . An equation of the tangent the parabola at $(8,4)$ is

$$
y-4=x-8
$$

or $\quad x-y-4=0$
Slope of the normal at $(8,4)$ is -1 . Therefore, equation of the normal at the given point is

$$
y-4=-(x-8)
$$

or $\quad x+y-12=0$
Example 2. Write equations of the tangent and normal to the conic $\frac{x^{2}}{8}+\frac{y^{2}}{9}=1$ at the point $\left(\frac{8}{3}, 1\right)$.

Solution: The given equation is

$$
9 x^{2}+8 y^{2}-72=0
$$

Differentiating (1) w.r.t. $x$, we have
This is slope of the tangent to (1) at $\left(\frac{8}{3}, 1\right)$.
Equation of the tangent at this point is
$y-1=-3 \cdot\left(x-\frac{8}{3}\right)=-3 x+8$ or $3 x+y-9=0$.
The normal at $\left(\frac{8}{3}, 1\right)$ has the slope $\frac{1}{3}$.
Equation of the normal is
$y-1=\frac{1}{3}\left(x-\frac{8}{3}\right)$ or $3 y-3=x-\frac{8}{3}$ or $3 x-9 y+1=0$

Theorem: To show that a straight line cuts a conic, in general, in two points and to find the condition that the line be a tangent to the conic.

Let a line $y=m x+c$ cut the conics
(i) $y=4 a x$
(ii) $\frac{x^{2}}{a^{2}}+\frac{y^{2}}{b^{2}}=1$
(iii) $\frac{x^{2}}{a^{2}}-\frac{y^{2}}{b^{2}}=1$

We shall discuss each case separately.
(i) The points of intersection of

$$
y=m x+c
$$

and $\quad y^{2}=4 a x$
are obtained by solving (1) and (2) simultaneously for $x$ and $y$. Inserting the value of $y$ from (1) into (2), we get

$$
(m x+c)^{2}=4 a x
$$

or $\quad m^{2} x^{2}+(2 m c-4 a) x+c^{2}=0$
which being a quadratic in $x$ gives two values of $x$. These values are the $x$ coordinates of the common points of (1) and (2). Setting these values in (1), we obtain the corresponding
ordinates of the points of intersection. Thus the line (1) cuts the parabola (2) in two points. In order that (1) is a tangent to (2), the points of intersection of a line and the parabola must be conicident. In this case, the roots of (3) should be real and equal.
This means that the discriminant of (3) is zero. Thus

$$
4(m c-2 a)^{2}-4 m^{2} c^{2}=0 \quad \text { i.e., } \quad-4 m c a+4 a^{2}=0
$$

or $\quad c=\frac{a}{m}$, is. the required condition for (1) to be a tangent to (2). Hence

$$
y=m x+\frac{a}{m} \text {, is a tangent to } y^{2}=4 a x \text { for all nonzero values of } m \text {. }
$$

(ii) To determine the points of intersection of

$$
y=m x+c
$$

and

$$
\frac{x^{2}}{a^{2}}+\frac{y^{2}}{b^{2}}=1
$$

we solve (1) and (2) simultaneously. Putting the value of $y$ from (1) into (2), we have

$$
\frac{x^{2}}{a^{2}}+\frac{(m x+c)^{2}}{b^{2}}=1
$$

or

$$
\left(a^{2} m^{2}+b^{2}\right) x^{2}+2 m c a^{2} x+a^{2} c^{2}-a^{2} b^{2}=0
$$

which is a quardratic in $x$ and it gives the abscissas of the two points where (1) and (2) intersect. The corresponding values of $y$ are obtained by setting the values of $x$ obtained from (3) into (1). Thus (1) and (2) intersect in two points. Now (1) is a tangent to (2) if the point of intersection is a single point.
This requires (3) to have equal roots. Hence (1) is a tangent to (2) if

$$
\left(2 m c a^{2}\right)^{2}-4\left(a^{2} m^{2}+b^{2}\right)\left(a^{2} c^{2}-a^{2} b^{2}\right)=0
$$

i.e., $\quad m^{2} c^{2} a^{2}-\left(a^{2} m^{2}+b^{2}\right)\left(c^{2}-b^{2}\right)=0$
or $\quad m^{2} c^{2} a^{2}-a^{2} m^{2} c^{2}+a^{2} m^{2} b^{2}-b^{2} c^{2}+b^{4}=0$
or $\quad c^{2}=a^{2} m^{2}+b^{2}$
or $\quad c=\sqrt{a^{2} m^{2} b^{2}}$.
Putting the value of $c$ into (1), we have

$$
\frac{x=m x \sqrt{a^{2} m^{2} b^{2}}}{x}
$$

which are tangents to (2) for all non-zero values of $m$.

(iii) We replace $b^{2}$ by $-b^{2}$ in (ii) and the line $y=m x+c$ is a tangent to

$$
\frac{x^{2}}{a^{2}}-\frac{y^{2}}{b^{2}}=1 \quad \text { if } \quad c=\sqrt{a^{2} m^{2}-b^{2}}
$$

Thus $y=m x \sqrt{a^{2} m^{2}-b^{2}}$ are tangents to the hyperbola: $\frac{x^{2}}{a^{2}}-\frac{y^{2}}{b^{2}}=1$ for all non-zero values of $m$.

Example 4. Find an equation of the tangent to the parabola $y^{2}=-6 x$ which is parallel to the line $2 x+y+1=0$. Also find the point of tangency.

Solution: Slope of the required tangent is $\mathrm{m}=-2$
In the parabola $y^{2}=-6 x$

$$
a=\frac{-6}{4}=\frac{-3}{2}
$$

Equation of the tangent is

$$
y=m x+\frac{a}{m}=-2 x+\frac{3}{4}
$$

i.e., $8 x+4 y-3=0$

Inserting the value of $y$ from (2) viz $y=\frac{-8 x+3}{4}$ into (1), we have

$$
\left(\frac{-8 x+3}{4}\right)^{2}=-6 x
$$

or $\quad 64 x^{2}-48 x+9=-96 x \quad$ or $\quad 64 x^{2}+48 x+9=0$
or $\quad(8 x+3)^{2}=0 \quad$ i.e., $\quad x=\frac{-3}{8}$
Putting this value of $x$ into (2), we get

$$
y=\frac{-8\left(\frac{-3}{8}\right)+3}{4}-\frac{3}{2}
$$

The point of tangency is $\left(\frac{-3}{8}, \frac{3}{2}\right)$.

## Example 5. Find equations of the tangents to the ellipse

$$
\frac{x^{2}}{128}+\frac{y^{2}}{18}=1
$$

which are parallel to the line $3 x+8 y+1=0$. Also find the points of contact.
Solution: The slope of the required tangents is $\frac{-3}{8}$. Equations of the tangents are

$$
y=\frac{-3}{8} x \pm \sqrt{\left(128\left(\frac{-3}{8}\right)^{2}+18=\frac{-3}{8} x \pm 6\right.}
$$

Thus the two tangents are

$$
3 x+8 y+48=0
$$

and $3 x+8 y-48=0$
We solve (1) and (3) simultaneously to find the point of contact. Inserting the value of $y$ from (3) into (1), we get

$$
\begin{aligned}
& \frac{x^{2}}{128}+\frac{\left(\frac{-3}{8} x+6\right)^{2}}{18}=1 \quad \text { or } \quad \frac{x^{2}}{128}+\frac{9}{64} \frac{x^{2}+36}{18}-\frac{9}{2} x \\
& \text { or } \quad \frac{x^{2}}{128}+\frac{x^{2}}{128}+2-\frac{x}{4}=1-\text { or }=\frac{x^{2}}{64}-\frac{x}{4} \quad 1 \quad 0 \\
& \text { or } \quad\left(\frac{x}{8}-1\right)^{2}=0 \quad \text { i.e., } x=8 \quad \text { and so } \quad \frac{-3}{8} x \quad 6 \quad 3
\end{aligned}
$$

Thus $(8,3)$ is the point of tangency of $(3)$.
It can be seen in a similar manner that point of contact of (2) is $(-8,-3)$.
Example 6. Show that the product of the distances from the foci to any tangent to the hyperbola

$$
\frac{x^{2}}{a^{2}}-\frac{y^{2}}{b^{2}}=1
$$

is constant.
Solution: The line

$$
y=m x \sqrt{a^{2} m^{2}-b^{2}}
$$

is a tangent to (1).
Foci of (1) are $F(-c, 0)$ and $F^{\prime}(c, 0)$.
Distance of $F(-c, 0)$ from (2) is

$$
d_{1}=\frac{\left|-c m+\sqrt{a^{2} m^{2}-b^{2}}\right|}{\sqrt{1+m^{2}}}
$$

Distance of $F^{\prime}(c, 0)$ from (2) is

$$
\begin{aligned}
& d_{2}=\frac{\left|c m+\sqrt{a^{2} m^{2}-b^{2}}\right|}{\sqrt{1+m^{2}}} \\
& d_{1} \times d_{2}=\frac{\left|a^{2} m^{2}-b^{2}-c^{2} m^{2}\right|}{1+m^{2}}=\frac{\left|a^{2} m^{2}-c^{2}+a^{2}-c^{2} m^{2}\right|}{1+m^{2}} \text { as } b^{2}=c^{2}-a^{2} \\
& \left|a^{2}-c^{2}\right| \\
& =c^{2}-a^{2} \quad \text { since } \quad c>a
\end{aligned}
$$

which is constant.

## Intersection of Two Coincs

Suppose we are given two conics

$$
\frac{x^{2}}{a^{2}} \cdot \frac{y^{2}}{b^{2}}=1
$$

and $y^{2}=4 a x$
To find the points common to both (1) and (2), we need to solve (1) and (2) simultaneously. It is known from algebra, that the simultaneous solution set of two equations of the second degree consists of four points. Thus two conics will always intersect in four points. These points may be all real and distinct, two real and two imaginary or all imaginary. Two or more points may also coincide. Two conics are said to touch each other if they intersect in two or more coincident points.

Example 7. Find the points of intersection of the ellipse

$$
\frac{x^{2}}{43 / 3} \cdot \frac{y^{2}}{43 / 4}=1-(1)=\text { and the hyperbola } \quad \frac{x^{2}}{7} \cdot \frac{y^{2}}{14} 1
$$

Also sketch the graph of the two conics.
Solution: The two equations may be written as

$$
3 x^{2}+4 y^{2}=43 \quad \text { (1) and } 2 x^{2}-y^{2}=14
$$

Multiplying (2) by 4 and adding the result to (1), we get

$$
11 x^{2}=99 \quad \text { or } \quad x= \pm 3
$$

Setting $x=3$ in to (2), we have $18-y^{2}=14$ or $y= \pm 2$
Thus $(3,2)$ and $(3,-2)$ are two points of intersection of the two conics
Putting $x=-3$ into (2), we get

$$
y= \pm 2
$$

Therefore $(-3,2)$ and $(-3,-2)$ are also points of intersection of (1) and (2). The four points of intersection are as shown in the figure.
Example 8. Find the points of intersection of the conics

$$
y=1+x^{2}
$$

and $\quad y=1+4 x-x^{2}$
Also draw the graph of the conics.
Solution. From (1), we have

$$
x=\sqrt{y-1}
$$

Inserting these values of $x$ into (2), we get

$$
y=1 \pm 4 \sqrt{y-1}-(y-1)
$$

or

$$
2 y-2= \pm 4 \sqrt{y-1} \quad \text { or } \quad(y-1)^{2}=4(y-1)
$$

or

$$
(y-1)(y-1-4)=0
$$

Therefore, $\quad y=1,5$
When $\quad y=1, x=0$
When $\quad y=5, x= \pm 2$

But $(-2,5)$ does not satisfy (2).
Thus $(0,1)$ and $(2,5)$ are the points of intersections of (1) and (2). $y=1+x^{2}$ is a parabola with vertex at $(0,1)$ and opening upward, $y=1+4 x-x^{2}$ may be written as $y-5=-(x-2)^{2}$ which is a parabola with vertex. $(2,5)$ and opening downward
Example 9. Find equations of the common tangents to the two conics

$$
\frac{x^{2}}{16}+\frac{y^{2}}{25}=1 \quad+\quad \text { and } \quad \frac{x^{2}}{25}-\frac{y^{2}}{9}=1
$$

Solution. The tangents with slope $m$, to the two conics are respectively given by

$$
y=\pi n x \sqrt{16 m^{2} 25} \quad \text { and } \quad y=\pi n x \sqrt{25 m^{2} 9}
$$

For a tangent to be common, we must have

$$
16 m^{2}+25=25 m^{2}+9
$$

or $\quad 9 m=16 \quad$ or $\quad m= \pm \frac{4}{3}$.
Using these values of $m$, equations of the four common tangents are:

$$
\pi=\frac{4}{3} x \sqrt{481}
$$

## EXERCISE 6.7

1. Find equations of the tangent and normal to each of the following at the indicated point:
(i) $y^{2}=4 a x$
(ii) $\frac{x^{2}}{a^{2}}+\frac{y^{2}}{b^{2}}=1$
(iii) $\frac{x^{2}}{a^{2}}-\frac{y^{2}}{b^{2}}=1$
at $\quad(a \cos \theta, b \sin \theta)$
at $\quad(a \sec \theta, b \tan \theta)$
2. Write equation of the tangent to the given conic at the indicated point
(i) $3 x^{2}=-16 y$ at the points whose ordinate is -3 .
(ii) $3 x^{2}-7 y^{2}=20$ at the points where $y=-1$.
(iii) $3 x^{2}-7 y^{2}+2 x-y-48=0$ at the point where $x=4$.
3. Find equations of the tangents to each of the following through the given point:
(i) $x^{2}+y^{2}=25$
(ii) $y^{2}=12 x$
(iii) $x^{2}-2 y^{2}=2$
through $(7,-1)$
through $(1,4)$
through $(1,-2)$
4. Find equations of the normals to the parabola $y^{2}=8 x$ which are parallel to the line $2 x+3 y=10$.
5. Find equations of the tangents to the ellipse $\frac{x^{2}}{4}+y^{2}=1$ which are parallel to the line $2 x-4 y+5=0$.
6. Find equations of the tangents to the conic $9 x^{2}-4 y^{2}=36$ parallel to $5 x-2 y+7=0$.
7. Find equations of the common tangents to the given conics
(i) $x^{2}=80 y$
(ii) $y^{2}=16 x$
and $x^{2}=2 y$
and $\quad \frac{x^{2}}{3}-\frac{y^{2}}{3}=1$
and $\quad x^{2}-y^{2}=1$
and $\quad 3 y^{2}-2 x^{2}=7$
and $\quad 9 x^{2}+y^{2}=124$
and $\quad x^{2}+y^{2}+y+8=0$