### 6.9 THE GENERAL EQUATION OF SECOND DEGREE

Standard equations of conic sections, namely circle, parabola, ellipse and hyperbola have already been studied in the previous sections. Now we shall take up the general equation of second degree viz.

$$
A x^{2}+B y^{2}+G x+F y+C=0
$$

The nature of the curve represented by (1) can be determined by examining the coefficients $A, B$ in the above equation. The following cases arise:
(i) If $A=B \neq 0$, equation (1) may be written as

$$
\begin{aligned}
& A\left(x^{2}+y^{2}\right)+G x+F y+C=0 \text { or } \quad x^{2}+y^{2}+\frac{G}{A} x+\frac{F}{A} y+\frac{C}{A}=0 \\
& \text { which represents a circle with centre at }\left(-\frac{G}{2 A},-\frac{F}{2 A}\right) \text { and radius } \sqrt{\frac{G^{2}}{4 A^{2}}+\frac{F^{2}}{4 A}-\frac{C}{A}}
\end{aligned}
$$

(ii) If $\quad A \neq B$ and both are of the same sign, then we have $\left(A x^{2}+G x\right)+\left(B y^{2}+F y\right)+C=0$
or $\quad A\left(x^{2}+\frac{G}{A} x+\frac{G^{2}}{4 A^{2}}\right)+B\left(y^{2}+\frac{F}{B} y+\frac{F^{2}}{4 B^{2}}\right)=\frac{G^{2}}{4 A}+\frac{F^{2}}{4 B}-C$
or $\quad A\left(x+\frac{G}{2 A}\right)^{2}+B\left(y+\frac{F}{2 B}\right)^{2}=\frac{G^{2}}{4 A}+\frac{F^{2}}{4 B}-C$
If we write $X \Leftrightarrow x \quad \frac{G}{4 A}, Y \quad y \quad \frac{F}{2 B}$, then (2) can be written as
$A X^{2}+B Y^{2}=\frac{G^{2}}{4 A}+\frac{F^{2}}{4 B}-C=K$ (say) or $\frac{X^{2}}{(\sqrt{K / A})^{2}}-\frac{Y^{2}}{(\sqrt{K / B})^{2}}, \quad 1$
which is standard equation of an ellipse in $X Y$-coordinate system.
(iii) If $A \neq B$ and both have opposite signs (say $A$ is positive and $B$ is negative),
we can write (1) as
or $\quad A\left(x^{2}+\frac{G}{A} x+\frac{G^{2}}{4 A^{2}}\right)-B^{\prime}\left(y^{2}-\frac{F}{B^{\prime}} y+\frac{F^{2}}{4 B^{\prime 2}}\right)=\frac{G^{2}}{4 A}-\frac{F^{2}}{4 B^{\prime}}-C=M$ (say)
or $\quad A\left(x+\frac{G}{2 A}\right)^{2}-B^{\prime}\left(y-\frac{F}{2 B^{\prime}}\right)^{2}=M$
or $\quad A X^{2}-B^{\prime} Y^{2}=M$, where $X=x-\frac{G}{2 A}, \quad Y \quad y-\frac{F}{2 B^{\prime}}$
or $\quad \frac{X^{2}}{(\sqrt{M / A})^{2}}-\frac{Y^{2}}{\left(\sqrt{M / B^{2}}\right)^{2}}=1$
and this is standard equation of a hyperbola in $X Y$-coordinates system.
(iv) If $A=0$ or $B=0$ (both cannot be zero since in that case the equation (1) reduces to a linear equation). Assume $A \neq 0$ and $B=0$.
The equation (1) becomes $A x^{2}+G x+F y+C=0$
or $\quad A\left(x^{2}+\frac{G}{A} x+\frac{G^{2}}{4 A^{2}}\right)=-F y-C+\frac{G^{2}}{4 A}$
or $\quad A\left(x+\frac{G}{2 A}\right)^{2}=-F\left(y+\frac{C}{F}-\frac{G^{2}}{4 A F}\right)$
or $\quad A X^{2}=-F Y$, where $X=x+\frac{G}{2 A}, \quad Y=y+\frac{C}{F}-\frac{G^{2}}{4 A F}$
which is standard equation of a parabola in $X Y$-coordinates system.
We summarize these results as under:
Let an equation of second degree be of the form $A x^{2}+B y^{2}+G x+F y+C=0$. It represents:
(i) a circle if $A=B \neq 0$
(ii) an ellipse if $A \neq B$ and both are of the same sign
(iii) a hyperbola if $A \neq B$ and both are of opposite signs
(iv) a parabola if either $A=0$ or $B=0$.