### 3.2.1 Some Standard Formulae for Anti-Derivatives

We give below a list of standard formulae for anti-derivatives which can be obtained from the corresponding formulae for derivatives:

## General Form

In formulae 1-7 and 10-14, a $\neq 0$

1. $\int(a x+b)^{n} d x=\frac{(a x+b)^{n-1}}{a(n+1)}+c,(n \neq-1) \quad\left\{x^{n} d x=\frac{x^{n-1}}{n+1}+c(n \neq-1)\right.$
2. $\int \sin (a x+b) d x=-\frac{1}{a} \cos (a x+b)+c \quad \int \sin x d x=\cos x$
3. $\int \cos (a x+b) d x=\frac{1}{a} \sin (a x+b)+c \quad \int \cos x d x=\sin x+c$
4. $\int \sec ^{2}(a x+b) d x=\frac{1}{a} \tan (a x+b)+c \quad \int \sec ^{2} x d x=\tan x$
5. $\int \operatorname{cosec}^{2}(a x+b) d x=-\frac{1}{a} \cot (a x+b)+c \quad \int \operatorname{cosec}^{2} x d x=\cot x$
6. $\int \sec (a x+b) \tan (a x+b) d x=\frac{1}{a} \sec (a x+b)+c \quad \int \sec x \tan x d x \neq \sec x$
7. $\int \operatorname{cosec}(a x+b) \cot (a x+b) d x=-\frac{1}{a} \operatorname{cosec}(a x+b)+c \quad \int \operatorname{cosec} \cot x d x=\operatorname{cosec} x$
8. $\int e^{2 x+a} d x=\frac{1}{\lambda} x e^{2 x+a}+c(\lambda \neq 0) \quad \int e^{x} d x=e^{x}+c$
9. $\int a^{2 x+a} d x=\frac{1}{\lambda \ln a} a^{2 x+a}+c .(a) 0, a \neq 1, \lambda \neq 0) \quad \int a^{2} d x=\frac{1}{\ln a} a^{2}+c .(a) 0, a \neq 1)$
10. $\int \frac{1}{a x+b} d x=\int(a x+b)^{-1} d x \quad\left\{\frac{1}{\lambda} d x=\ln |x|+c, x \neq 0\right.$

$$
=\frac{1}{a} \ln |a x+b|+c,(a x+b \neq 0)
$$

11. $\int \tan (a x+b) d x=\frac{1}{a} \ln |\sec (a x+b)|+c \quad \int \tan x d x=\ln |\sec (x)|+c$

$$
\Rightarrow \frac{1}{a} \ln |\cos (\boldsymbol{a} x \quad \boldsymbol{b})| \quad c \quad=\ln |\cos x| \quad c
$$

12. $\int \cot (a x+b) d x=\frac{1}{a} \ln |\sin (a x+b)|+c \quad \int \cot x d x=\ln |\sin x|+c$
13. $\int \sec (a x+b) d x=\frac{1}{a} \ln |\sec (a x+b)+\tan (a x+b)|+c \quad \int \sec x d x=\ln |\sec x+\tan x|+c$
14. $\int \operatorname{cosec}(a x+b) d x=\frac{1}{a} \ln |\operatorname{cosec}(a x+b)-\cot (a x+b)|+c \quad \int \operatorname{cosec} x d x=\ln |\operatorname{cosec} x-\cot x|+c$

These formulae can be verified by showing that the derivative of the right hand side of each with respect to $x$ is equal to the corresponding integrand.

## Examples:

1. $\int x^{5} d x=\frac{x^{5-1}}{5+1}+c=\frac{x^{6}}{6}+c \quad\left(1-\frac{d}{d x}\left(\frac{1}{6} x^{6}\right)\right)=\frac{1}{6} d x\left(x^{6}\right)=\frac{1}{6} \cdot 6 x^{6-1}=x^{5}$
2. $\int \frac{1}{\sqrt{x^{3}}} d x=\int x^{-\frac{1}{2}} d x=\frac{x^{-\frac{1}{2}-1}}{-\frac{3}{2}+1} \quad\left[1-\frac{d}{d x}\left(\frac{-2}{\sqrt{x}}\right)=-2 \frac{d}{d x}(x)^{\frac{1}{2}}\right]$

$$
=\frac{x^{\frac{1}{2}}}{-\frac{1}{2}}+c=-\frac{2}{\sqrt{x}}+c \quad=-2 \cdot\left(-\frac{1}{2}\right) x^{\frac{1}{2}+}=x^{\frac{-1}{2}} \frac{1}{\sqrt{x^{2}}}
$$

3. $\int \frac{1}{(2 x+3)^{4}} d \dot{x}=(\varnothing x \quad 3)^{-4} d x \quad\left(\because \frac{d}{d x}\left(\frac{1}{6(2 x+3)^{2}}\right)\right)$
$=\frac{(2 x+3)^{-4+1}}{2(-4+1)}+c=\frac{(2 x+3)^{-3}}{-6}+c \quad=\frac{1}{6} \frac{d}{d x}\left((2 x \quad 3)^{-3}\right)$
$=\frac{1}{6(2 x+3)^{2}} \quad c \quad=-\frac{1}{6}(-3)(2 x+3)^{-3-1}(2)=\frac{1}{(2 x+3)^{4}}$
4. $\int \cos 2 x d x=\frac{\sin 2 x}{2}+c=\frac{1}{2} \sin 2 x+c \quad\left(\because \frac{d}{d x}\left(\frac{1}{2} \sin 2 x\right)=\frac{1}{2} \frac{d}{d x}(\sin 2 x)\right)$
$=\frac{1}{2}(\cos 2 x) \times 2=\cos 2 x$
5. $\int \sin 3 x d x=\frac{-\cos 3 x}{3}+c=\frac{1}{3} \cos 3 x+c \quad\left(\because \frac{d}{d x}\left(-\frac{1}{3} \cos 3 x\right)=\frac{1}{3} \frac{d}{d x}(\cos 3 x)\right)$
6. $\int \cos \sec ^{2} x d x=\operatorname{sec} x \quad c \quad\left(\because \frac{d}{d x}(-\cot x)=-\left(-\cos \sec ^{2} x\right)=\cos \sec ^{2} x\right)$
7. $\int \sec 5 x \tan 5 x d x=\frac{\sec 5 x}{5} \quad c \quad\left(\because \frac{d}{d x}\left(\frac{\sec 5 x}{5}\right)\right)=\frac{1}{5}(\operatorname{sen} 5 x \tan 5 x) \quad 5 \quad \sec 5 x \tan 5 x$
8. $\int e^{a x+b} d x=\frac{e^{a x+b}}{a}+c \quad\left(\because \frac{d}{d x}\left(\frac{e^{a x+b}}{a}\right)=\frac{1}{a}\left(e^{a x+b} \times a\right)=e^{a x+b}\right)$
9. $\int 3^{3 / 2} d x=\frac{3^{3 / 2}}{\lambda \ln 3}+c \quad\left(\because \frac{d}{d x}\left(\frac{3^{3 / 2}}{\lambda \ln 3}\right)=\frac{1}{\lambda \ln 3}\left(3^{3 / 2}(\ln 3) \lambda\right) \quad 3^{3 / 2}\right)$
10. $\int \frac{1}{a x+b} d \dot{x}=(\omega x \quad b)^{-1} d x \quad\left(\because \frac{d}{d x}\left(\frac{1}{a} \ln (a x+b)=\frac{1}{a} \frac{1}{a x+b} \cdot a=\frac{1}{a x+b}\right)\right)$
$=\frac{1}{a} \ln (a x+b)+c \cdot(a x+b>0)$
11. $\int \frac{1}{\sqrt{x^{2}+a^{2}}} d x=\ln \left(x+\sqrt{x^{2}+a^{2}}\right)+c \quad\left(\because \frac{d}{d x}\left(\ln (x+\sqrt{x^{2}+a^{2}})\right)=\frac{1}{x+\sqrt{x^{2}+a^{2}}}\left(1+\frac{1}{2 \sqrt{x^{2}+a^{2}}}+2 x\right)\right)$

$$
\frac{1}{x+\sqrt{x^{2}+a^{2}}}=\frac{\sqrt{x^{2}+a^{2}}+x}{\sqrt{x^{2}+a^{2}}}=\frac{1}{\sqrt{x^{2}+a^{2}}}
$$