### 3.4.1 Rational Equations Reducible to the Quadratic Equation

A rational equation is an equation containing one or more rational expressions, where rational expressions typically contain a variable in the denominator.
Example 7 Solve $\frac{1}{x}+\frac{2}{x+1}=1, x \neq 0, x \neq-1$
Solution $\frac{1}{x}+\frac{2}{x+1}=1$
Multiplying both sides by $x(x+1)$, we have

$$
\begin{aligned}
(x+1)+2 x & =x(x+1) \\
x+1+2 x & =x^{2}+x \\
3 x+1 & =x^{2}+x \\
x^{2}+x-3 x-1 & =0 \\
x^{2}-2 x-1 & =0 \\
x & =\frac{-(-2) \pm \sqrt{(-2)^{2}-4(1)(-1)}}{2(1)} \\
& =\frac{2 \pm \sqrt{4+4}}{2} \\
x & =\frac{2 \pm \sqrt{8}}{2} \\
& =\frac{2 \pm 2 \sqrt{2}}{2} \\
& =1 \pm \sqrt{2}
\end{aligned}
$$

Hence, Solution Set $=\{1 \pm \sqrt{2}\}$

# 3.4.2 Radical Equations Reducible to the Quadratic Equation

Equations involving radical expressions of the variable are called radical equations. To solve a radical equation, we first obtain an equation free from radicals. Every solution of radical equation is also a solution of the radical-free equation but the new equation has solutions that are not solutions of the original radical equation. Such extra solutions (roots) are called extraneous roots.
Example 8 Solve $\sqrt{x+8}+\sqrt{x+3}=\sqrt{12 x+13}$
Solution $\sqrt{x+8}+\sqrt{x+3}=\sqrt{12 x+13}$
Squaring both sides, we get

$$
\begin{aligned}
x+8+x+3+2(\sqrt{x+8})(\sqrt{x+3}) & =12 x+13 \\
2(\sqrt{x+8})(\sqrt{x+3}) & =10 x+2 \\
\Rightarrow \quad \sqrt{(x+8)(x+3)} & =5 x+1
\end{aligned}
$$

Squaring again, we have

$$
\begin{aligned}
x^{2}+11 x+24 & =25 x^{2}+10 x+1 \\
\Rightarrow \quad 24 x^{2}-x-23 & =0 \\
\Rightarrow \quad(24 x+23)(x-1) & =0 \\
x & =-\frac{23}{24} \text { or } x=1
\end{aligned}
$$

On checking we find that $-\frac{23}{24}$ is an extraneous root. Hence solution set $=\{1\}$